@prefix : <http://emmo.info/emmo/domain/mechanical-testing#> .
@prefix owl: <http://www.w3.org/2002/07/owl#> .
@prefix rdf: <http://www.w3.org/1999/02/22-rdf-syntax-ns#> .
@prefix xml: <http://www.w3.org/XML/1998/namespace> .
@prefix xsd: <http://www.w3.org/2001/XMLSchema#> .
@prefix emmo: <http://emmo.info/emmo#> .
@prefix rdfs: <http://www.w3.org/2000/01/rdf-schema#> .
@prefix skos: <http://www.w3.org/2004/02/skos/core#> .
@prefix chameo: <http://emmo.info/emmo/domain/chameo/chameo#> .
@prefix dcterms: <http://purl.org/dc/terms/> .

<http://emmo.info/emmo/domain/mechanical-testing/indentation> a owl:Ontology ;
	owl:versionIRI <http://emmo.info/emmo/domain/mechanical-testing/1.0.0/indentation> ;
	owl:imports <http://emmo.info/emmo/domain/mechanical-testing/mechanical-testing> ;
	dcterms:creator "Adham Hashibon" , "Yoav Nahshon" ;
	owl:versionInfo "1.0.0" ;
	dcterms:contributor "Goldbeck Consulting Ltd (UK)" ;
	dcterms:publisher "EMMC ASBL" ;
	dcterms:title "Domain Mechanical Testing"@en ;
	rdfs:comment "This ontology is a joint colaboration between different projects: OYSTER, UrWerk and MarketPlace."@en ;
	dcterms:contributor "Fraunhofer IWM, DE" ;
	dcterms:creator "Joana Francisco Morgado" ;
	dcterms:license "https://creativecommons.org/licenses/by/4.0/legalcode" ;
	dcterms:creator "Daniele Toti" , "Gerhard Goldbeck" ;
	dcterms:abstract "A domain ontology for Mechanical Testing based on EMMO."@en .
# 
# 
# #################################################################
# #
# #    Classes
# #
# #################################################################
# 
# 
# http://emmo.info/emmo/domain/mechanical-testing#EMMO_03e264fd_ee9f_4ac0_a9f4_b0a975ddaded

:EMMO_03e264fd_ee9f_4ac0_a9f4_b0a975ddaded a owl:Class ;
	rdfs:subClassOf emmo:EMMO_494b372c_cfdf_47d3_a4de_5e037c540de8 , _:genid1 .

_:genid1 a owl:Restriction ;
	owl:onProperty emmo:EMMO_9380ab64_0363_4804_b13f_3a8a94119a76 ;
	owl:someValuesFrom :EMMO_f2d6622f_83f7_4b66_b75c_d4576ad5d986 .

:EMMO_03e264fd_ee9f_4ac0_a9f4_b0a975ddaded rdfs:comment "The hardware set consisting of the indenter column, indenter tip, the support springs, the displacement capacitive sensor, the actuation coil the metal case and the interface with the control electronics." ;
	skos:prefLabel "IndenterHead"@en .
# 
# http://emmo.info/emmo/domain/mechanical-testing#EMMO_03ed6a50_3b04_4189_a939_dad066ece197

:EMMO_03ed6a50_3b04_4189_a939_dad066ece197 a owl:Class ;
	rdfs:subClassOf emmo:EMMO_d4f7d378_5e3b_468a_baa1_a7e98358cda7 , :EMMO_347cecd5_9d8b_42cb_b12b_76c6fa4090e5 ;
	rdfs:comment "The time constant used to measure the Dynamic displacement (time over which the RMS value of the displacement is computed). Generally equivalent to at least five waves at the target frequency and being an integer number of waves. This dramatically reduces noise ." ;
	skos:prefLabel "DynamicTimeConstant"@en .
# 
# http://emmo.info/emmo/domain/mechanical-testing#EMMO_0ae01f99_b2ed_4dd0_959d_60baad0ab475

:EMMO_0ae01f99_b2ed_4dd0_959d_60baad0ab475 a owl:Class ;
	rdfs:subClassOf emmo:EMMO_79751276_b2d0_4e2f_bbd4_99d412f43d55 ;
	rdfs:comment "The amplitude of the displacement value oscillation reading while in contact with the sample, with respect to its quasi static value." ;
	skos:prefLabel "AmplitudeOfOscillatoryDepthReading"@en .
# 
# http://emmo.info/emmo/domain/mechanical-testing#EMMO_10e7f26e_4cb6_4fb8_84e8_f90fec466e75

:EMMO_10e7f26e_4cb6_4fb8_84e8_f90fec466e75 a owl:Class ;
	rdfs:subClassOf emmo:EMMO_d4f7d378_5e3b_468a_baa1_a7e98358cda7 , :EMMO_347cecd5_9d8b_42cb_b12b_76c6fa4090e5 ;
	rdfs:comment "The time over which the drift rate is measured." ;
	skos:prefLabel "DriftDeterminationTime"@en .
# 
# http://emmo.info/emmo/domain/mechanical-testing#EMMO_19afc39b_eb5c_46e0_b880_8e08ec831ebc

:EMMO_19afc39b_eb5c_46e0_b880_8e08ec831ebc a owl:Class ;
	rdfs:subClassOf :EMMO_a30a7cdc_f652_4b01_b8c2_cd056f3e3d85 , _:genid2 .

_:genid2 a owl:Restriction ;
	owl:onProperty emmo:EMMO_9380ab64_0363_4804_b13f_3a8a94119a76 ;
	owl:someValuesFrom :EMMO_de2e853c_c30e_4710_9c8a_671dba758955 .

:EMMO_19afc39b_eb5c_46e0_b880_8e08ec831ebc skos:prefLabel "IndentationMachine"@en .
# 
# http://emmo.info/emmo/domain/mechanical-testing#EMMO_2ebac53b_0902_43c3_abe5_fc110fbec98f

:EMMO_2ebac53b_0902_43c3_abe5_fc110fbec98f a owl:Class ;
	rdfs:subClassOf :EMMO_4877705b_70a3_453e_b7f2_510965fa2ff7 , :EMMO_ca42ed31_3983_4e1a_84f9_a84cab2cdb59 ;
	rdfs:comment "The displacement difference between the beginning of the pull-off phenomenon and its end during an adhesion experiment." ;
	skos:prefLabel "PulloffDisplacement"@en .
# 
# http://emmo.info/emmo/domain/mechanical-testing#EMMO_301113f2_d390_4b1d_8cff_4d4ef9c1fc55

:EMMO_301113f2_d390_4b1d_8cff_4d4ef9c1fc55 a owl:Class ;
	rdfs:subClassOf :EMMO_ba4f6d96_699f_48ba_a432_6676521587f1 ;
	skos:prefLabel "MaximumIndentationTime"@en .
# 
# http://emmo.info/emmo/domain/mechanical-testing#EMMO_3226bd7c_b9d8_436d_ae5f_8a69a92ea128

:EMMO_3226bd7c_b9d8_436d_ae5f_8a69a92ea128 a owl:Class ;
	rdfs:subClassOf emmo:EMMO_79751276_b2d0_4e2f_bbd4_99d412f43d55 ;
	rdfs:comment "Constant strain rate testing involves the application of load so that the depth measurements follow a pre-defined relationship. Set the loading rate to give a constant rate of strain within the specimen material." ;
	skos:prefLabel "ConstantStrainRate"@en .
# 
# http://emmo.info/emmo/domain/mechanical-testing#EMMO_347cecd5_9d8b_42cb_b12b_76c6fa4090e5

:EMMO_347cecd5_9d8b_42cb_b12b_76c6fa4090e5 a owl:Class ;
	rdfs:subClassOf emmo:EMMO_d8d2144e_5c8d_455d_a643_5caf4d8d9df8 ;
	rdfs:label "IndentationMethodSpecification"@de .
# 
# http://emmo.info/emmo/domain/mechanical-testing#EMMO_37056c17_4800_42c6_8827_1873cb7e417d

:EMMO_37056c17_4800_42c6_8827_1873cb7e417d a owl:Class ;
	rdfs:subClassOf emmo:EMMO_b7bcff25_ffc3_474e_9ab5_01b1664bd4ba , _:genid3 .

_:genid3 a owl:Restriction ;
	owl:onProperty _:genid4 .

_:genid4 owl:inverseOf emmo:EMMO_e1097637_70d2_4895_973f_2396f04fa204 .

_:genid3 owl:someValuesFrom :EMMO_1cbdb7f5_47e4_468a_8d87_b25093803b8e .

:EMMO_37056c17_4800_42c6_8827_1873cb7e417d rdfs:label "SpecimenProperty"@de .
# 
# http://emmo.info/emmo/domain/mechanical-testing#EMMO_3fdd2c2f_762b_4d0f_b883_4cf47a2da2f9

:EMMO_3fdd2c2f_762b_4d0f_b883_4cf47a2da2f9 a owl:Class ;
	rdfs:subClassOf emmo:EMMO_1f087811_06cb_42d5_90fb_25d0e7e068ef , :EMMO_4877705b_70a3_453e_b7f2_510965fa2ff7 ;
	rdfs:comment "The force needed to overcome the adhesion phenomena between indenter tip and material under investigation." ;
	skos:prefLabel "PulloffForce"@en .
# 
# http://emmo.info/emmo/domain/mechanical-testing#EMMO_4877705b_70a3_453e_b7f2_510965fa2ff7

:EMMO_4877705b_70a3_453e_b7f2_510965fa2ff7 a owl:Class ;
	rdfs:subClassOf :EMMO_37056c17_4800_42c6_8827_1873cb7e417d ;
	rdfs:label "IndentationSpecimenProperty"@de .
# 
# http://emmo.info/emmo/domain/mechanical-testing#EMMO_68856430_66a2_49fb_b93f_e7124effb6bd

:EMMO_68856430_66a2_49fb_b93f_e7124effb6bd a owl:Class ;
	rdfs:subClassOf emmo:EMMO_cd2cd0de_e0cc_4ef1_b27e_2e88db027bac , :EMMO_347cecd5_9d8b_42cb_b12b_76c6fa4090e5 ;
	rdfs:comment "The distance from the last known value of the displacement associated with the surface at which the system will establish the “Approach Velocity” and start looking for the surface." ;
	skos:prefLabel "SurfaceApproachDistance"@en .
# 
# http://emmo.info/emmo/domain/mechanical-testing#EMMO_68efbbca_549a_4209_bdfc_cf0ddfd27dc9

:EMMO_68efbbca_549a_4209_bdfc_cf0ddfd27dc9 a owl:Class ;
	rdfs:subClassOf emmo:EMMO_0329f1f5_8339_4ce4_8505_a264c6d606ba , :EMMO_347cecd5_9d8b_42cb_b12b_76c6fa4090e5 ;
	rdfs:comment "The velocity of the probe as it approaches the surface." ;
	skos:prefLabel "SurfaceApproachVelocity"@en .
# 
# http://emmo.info/emmo/domain/mechanical-testing#EMMO_6a8bfa0e_ef96_4f38_b892_40389eb7d69d

:EMMO_6a8bfa0e_ef96_4f38_b892_40389eb7d69d a owl:Class ;
	rdfs:subClassOf :EMMO_347cecd5_9d8b_42cb_b12b_76c6fa4090e5 , :EMMO_ee09aa64_f477_4e8f_8b0c_f5d30177ba8d ;
	rdfs:comment "The targeted maximum depth. The experiment will stop loading at this point or if the maximum target load is reached." ;
	skos:prefLabel "TargetDepth"@en .
# 
# http://emmo.info/emmo/domain/mechanical-testing#EMMO_73e0c7f8_20db_46c7_af69_22ad5616f8dc

:EMMO_73e0c7f8_20db_46c7_af69_22ad5616f8dc a owl:Class ;
	rdfs:subClassOf :EMMO_347cecd5_9d8b_42cb_b12b_76c6fa4090e5 ;
	rdfs:comment "The displacement resolution is typically found by dividing the maximum displacement voltage reading by the number of bits in the data acquisition system." ;
	skos:prefLabel "DisplacementResolution"@en .
# 
# http://emmo.info/emmo/domain/mechanical-testing#EMMO_76dba92f_a761_409f_83d8_5a0c9c73b349

:EMMO_76dba92f_a761_409f_83d8_5a0c9c73b349 a owl:Class ;
	rdfs:subClassOf chameo:DataPostProcessing ;
	skos:prefLabel "IndentationTestPostProcessing"@en .
# 
# http://emmo.info/emmo/domain/mechanical-testing#EMMO_7aa20434_165d_414f_a945_b57bd849e43b

:EMMO_7aa20434_165d_414f_a945_b57bd849e43b a owl:Class ;
	rdfs:subClassOf emmo:EMMO_4bc29b0f_8fcc_4026_a291_f9774a66d9b8 ;
	rdfs:comment "The area function that describes the geometry according to which the indenter tip diamond end is cut: three sided pyramids, four sided pyramids, wedges, cones, cylinders or spheres. The tip end of the indenter can be made sharp, flat, or rounded to a cylindrical or spherical shape. All these features of the indenter tip can be described with a mathematical function." ;
	skos:prefLabel "IndenterTipAreaFunction"@en .
# 
# http://emmo.info/emmo/domain/mechanical-testing#EMMO_8aa746fa_0cfa_4be7_9e5b_a691a860032e

:EMMO_8aa746fa_0cfa_4be7_9e5b_a691a860032e a owl:Class ;
	rdfs:subClassOf :EMMO_347cecd5_9d8b_42cb_b12b_76c6fa4090e5 ;
	rdfs:comment "In load frames of finite stiffness, the load applied via the indenter induces displacement in both the sample and the load frame. Frame compliance must be identified and subtracted from the total indenter displacement to account properly for sample deformation." ;
	skos:prefLabel "LoadFrameCompliance"@en .
# 
# http://emmo.info/emmo/domain/mechanical-testing#EMMO_9d621c9b_9c52_4084_af20_b2dfda89fe6c

:EMMO_9d621c9b_9c52_4084_af20_b2dfda89fe6c a owl:Class ;
	rdfs:subClassOf emmo:EMMO_463bcfda_867b_41d9_a967_211d4d437cfb , _:genid5 .

_:genid5 a owl:Restriction ;
	owl:onProperty emmo:EMMO_ae2d1a96_bfa1_409a_a7d2_03d69e8a125a ;
	owl:someValuesFrom :EMMO_19afc39b_eb5c_46e0_b880_8e08ec831ebc .

:EMMO_9d621c9b_9c52_4084_af20_b2dfda89fe6c rdfs:subClassOf _:genid6 .

_:genid6 a owl:Restriction ;
	owl:onProperty :EMMO_a079cf37_e495_41f1_af01_d544e886eacb ;
	owl:someValuesFrom :EMMO_376c6456_5601_41c2_987c_3063f14408d4 .

:EMMO_9d621c9b_9c52_4084_af20_b2dfda89fe6c rdfs:subClassOf _:genid7 .

_:genid7 a owl:Restriction ;
	owl:onProperty :EMMO_a079cf37_e495_41f1_af01_d544e886eacb ;
	owl:someValuesFrom :EMMO_ca42ed31_3983_4e1a_84f9_a84cab2cdb59 .

:EMMO_9d621c9b_9c52_4084_af20_b2dfda89fe6c rdfs:subClassOf _:genid8 .

_:genid8 a owl:Restriction ;
	owl:onProperty :EMMO_a079cf37_e495_41f1_af01_d544e886eacb ;
	owl:someValuesFrom :EMMO_ee09aa64_f477_4e8f_8b0c_f5d30177ba8d .

:EMMO_9d621c9b_9c52_4084_af20_b2dfda89fe6c skos:prefLabel "IndentationMeasurement"@en .
# 
# http://emmo.info/emmo/domain/mechanical-testing#EMMO_a1c92b74_411d_414c_85e0_36ddd8c8afb6

:EMMO_a1c92b74_411d_414c_85e0_36ddd8c8afb6 a owl:Class ;
	rdfs:subClassOf emmo:EMMO_d4f7d378_5e3b_468a_baa1_a7e98358cda7 , :EMMO_347cecd5_9d8b_42cb_b12b_76c6fa4090e5 ;
	rdfs:comment "This is the time specified to linearly reduce the load on the contact form it’s maximum value to zero." ;
	skos:prefLabel "TargetUnloadTime"@en .
# 
# http://emmo.info/emmo/domain/mechanical-testing#EMMO_ba4f6d96_699f_48ba_a432_6676521587f1

:EMMO_ba4f6d96_699f_48ba_a432_6676521587f1 a owl:Class ;
	rdfs:subClassOf emmo:EMMO_d4f7d378_5e3b_468a_baa1_a7e98358cda7 , :EMMO_347cecd5_9d8b_42cb_b12b_76c6fa4090e5 ;
	rdfs:comment "This is the average time of a typical indentation cycle from load to full unload." ;
	skos:prefLabel "IndentationTime"@en .
# 
# http://emmo.info/emmo/domain/mechanical-testing#EMMO_c16d56fc_ad1f_420d_9d61_edbe4a28136a

:EMMO_c16d56fc_ad1f_420d_9d61_edbe4a28136a a owl:Class ;
	owl:equivalentClass _:genid9 .

_:genid9 a owl:Restriction ;
	owl:onProperty emmo:EMMO_ae2d1a96_bfa1_409a_a7d2_03d69e8a125a ;
	owl:someValuesFrom _:genid10 .

_:genid10 owl:intersectionOf _:genid12 .

_:genid12 a rdf:List ;
	rdf:first :EMMO_76dba92f_a761_409f_83d8_5a0c9c73b349 ;
	rdf:rest _:genid11 .

_:genid11 a rdf:List ;
	rdf:first :EMMO_9d621c9b_9c52_4084_af20_b2dfda89fe6c ;
	rdf:rest rdf:nil .

_:genid10 a owl:Class .

:EMMO_c16d56fc_ad1f_420d_9d61_edbe4a28136a rdfs:subClassOf :EMMO_0f73321c_c4fd_40ed_9b58_eccd9b7d8e15 , _:genid13 .

_:genid13 a owl:Restriction ;
	owl:onProperty emmo:EMMO_ae2d1a96_bfa1_409a_a7d2_03d69e8a125a ;
	owl:someValuesFrom :EMMO_76dba92f_a761_409f_83d8_5a0c9c73b349 .

:EMMO_c16d56fc_ad1f_420d_9d61_edbe4a28136a rdfs:subClassOf _:genid14 .

_:genid14 a owl:Restriction ;
	owl:onProperty emmo:EMMO_ae2d1a96_bfa1_409a_a7d2_03d69e8a125a ;
	owl:someValuesFrom :EMMO_9d621c9b_9c52_4084_af20_b2dfda89fe6c .

:EMMO_c16d56fc_ad1f_420d_9d61_edbe4a28136a rdfs:comment "A single indentation experiment." ;
	skos:prefLabel "IndentationTest"@en .
# 
# http://emmo.info/emmo/domain/mechanical-testing#EMMO_de2e853c_c30e_4710_9c8a_671dba758955

:EMMO_de2e853c_c30e_4710_9c8a_671dba758955 a owl:Class ;
	rdfs:subClassOf emmo:EMMO_494b372c_cfdf_47d3_a4de_5e037c540de8 , _:genid15 .

_:genid15 a owl:Restriction ;
	owl:onProperty emmo:EMMO_9380ab64_0363_4804_b13f_3a8a94119a76 ;
	owl:someValuesFrom :EMMO_03e264fd_ee9f_4ac0_a9f4_b0a975ddaded .

:EMMO_de2e853c_c30e_4710_9c8a_671dba758955 skos:prefLabel "IndenterDevice"@en .
# 
# http://emmo.info/emmo/domain/mechanical-testing#EMMO_ebb3c390_173a_4c23_a338_12b6a75ddab2

:EMMO_ebb3c390_173a_4c23_a338_12b6a75ddab2 a owl:Class ;
	rdfs:subClassOf :EMMO_347cecd5_9d8b_42cb_b12b_76c6fa4090e5 ;
	rdfs:comment "The noise floor in the displacement measurement system will determine what the minimum useable indentation depth." ;
	skos:prefLabel "DisplacementNoiseFloor"@en .
# 
# http://emmo.info/emmo/domain/mechanical-testing#EMMO_ecc66886_7f39_42a5_99f4_c260b74ed7f5

:EMMO_ecc66886_7f39_42a5_99f4_c260b74ed7f5 a owl:Class ;
	rdfs:subClassOf :EMMO_c16d56fc_ad1f_420d_9d61_edbe4a28136a ;
	rdfs:comment "An indentation test where only the maximum applied load is controlled." ;
	skos:prefLabel "StaticIndentation"@en .
# 
# http://emmo.info/emmo/domain/mechanical-testing#EMMO_f2d6622f_83f7_4b66_b75c_d4576ad5d986

:EMMO_f2d6622f_83f7_4b66_b75c_d4576ad5d986 a owl:Class ;
	rdfs:subClassOf emmo:EMMO_494b372c_cfdf_47d3_a4de_5e037c540de8 , _:genid16 .

_:genid16 a owl:Restriction ;
	owl:onProperty emmo:EMMO_24c71baf_6db6_48b9_86c8_8c70cf36db0c ;
	owl:someValuesFrom :EMMO_7aa20434_165d_414f_a945_b57bd849e43b .

:EMMO_f2d6622f_83f7_4b66_b75c_d4576ad5d986 rdfs:subClassOf _:genid17 .

_:genid17 a owl:Restriction ;
	owl:onProperty emmo:EMMO_e1097637_70d2_4895_973f_2396f04fa204 ;
	owl:someValuesFrom :EMMO_b50db598_cfea_4582_9168_46fbc0b9ec4f .

:EMMO_f2d6622f_83f7_4b66_b75c_d4576ad5d986 rdfs:comment """The probe used during an indentation test, generally composed by three parts:
1.	The diamond;
2.	The holder;
3.	The bond;""" ;
	skos:prefLabel "IndenterTip"@en .
# 
# Generated by the OWL API (version 4.2.8.20170104-2310) https://github.com/owlcs/owlapi
